examples/mutsum/MutFG.v
@@ -1,0 +1,43 @@
+Require Import Coqlib.
+Require Import ITreelib.
+Require Import Universe.
+Require Import STS.
+Require Import Behavior.
+Require Import ModSem.
+Require Import Skeleton.
+Require Import PCM.
+Require Import Hoare.
+Require Import MutHeader.
+Require Import MutF1 MutG1.
+
+Generalizable Variables E R A B C X Y Σ.
+
+Set Implicit Arguments.
+
+
+
+Section PROOF.
+
+  Context `{Σ: GRA.t}.
+
+  Definition FG1: Mod.t := Mod.add F G.
+
+  Definition FG2: Mod.t := {|
+    Mod.get_modsem := fun _ => {|
+        ModSem.fnsems := List.map (fun '(fn, body) => (fn, fun_to_src body)) (FFtb ++ GFtb);
+        ModSem.initial_mrs := [];
+      |};
+    Mod.sk := Sk.unit;
+  |}
+  .
+
+  Theorem correct: Beh.of_program (Mod.interp FG1) <1= Beh.of_program (Mod.interp FG2).
+  Proof.
+    ii.
+    eapply adequacy_type with (ftb:=FFtb++GFtb) in PR. cbn in *.
+    rp; try apply PR; cycle 1.
+    { refl. }
+    clear PR. f_equal.
+  Qed.
+
+End PROOF.
